Partial implementation of [dll_split_using] iface.
Some parts of proof TBD. Looks like all the nice auto triggering
lemmas that I'd set up don't trigger at all for this one. I'll need to
manually call out to the requisite functions.

ind/DoublyLinkedListIface.fst
@@ -594,6 +594,52 @@ let dll_append #t d1 d2 =
 
 #reset-options
 
+#set-options "--z3rlimit 100 --max_fuel 2 --max_ifuel 1"
+
+let dll_split_using #t d1 d2 n =
+  let h00 = HST.get () in
+  HST.push_frame ();
+  let h0 = HST.get () in
+  let y1, y2 = DLL.dll_split_using (!*d1) n in
+  let h0' = HST.get () in
+  d1 *= y1;
+  let h0'' = HST.get () in
+  d2 *= y2;
+  let h1 = HST.get () in
+  assert (B.loc_buffer d1 `B.loc_disjoint` DLL.dll_fp0 (d1@h0));
+  assert (DLL.dll_fp0 (d1@h0) `B.loc_includes` DLL.dll_fp0 y1);
+  FStar.Classical.arrow_to_impl
+  #(L.length (G.reveal (d1@h0).DLL.nodes) >= 2)
+  #(DLL.dll_fp0 (d1@h0) `B.loc_includes` B.loc_buffer ((d1@h0).DLL.ltail@h0).DLL.blink)
+    (fun _ ->
+       DLL.extract_nodelist_conn h0 (G.reveal (d1@h0).DLL.nodes) (L.length (G.reveal (d1@h0).DLL.nodes) - 2);
+       DLL.extract_nodelist_fp0 (G.reveal (d1@h0).DLL.nodes) (L.length (G.reveal (d1@h0).DLL.nodes) - 2);
+       L.lemma_unsnoc_is_last (G.reveal (d1@h0).DLL.nodes));
+  _lemma_prev_node_in_list h0 n d1;
+  _lemma_node_in_list_or_null_is_included ((n@h0).DLL.blink) (G.reveal (d1@h0).DLL.nodes);
+  _lemma_node_in_list_is_included n (G.reveal (d1@h0).DLL.nodes);
+  assert (B.loc_buffer d1 `B.loc_disjoint` DLL.dll_fp0 (d1@h0'));
+  _lemma_unchanged_node_vals_stays_valid0 h0' h0'' d1;
+  _lemma_unchanged_node_vals_transitive h0 h0' h0'' (as_list h0 d1);
+  //
+  assume (unchanged_node_vals h0'' h1 (as_list h0 d1));
+  assert (_pred_nl_disjoint h0 (as_list h0 d1));
+  assert (_pred_nl_disjoint h0 (as_list h1 d1));
+  assert (_pred_nl_disjoint h0 (as_list h1 d2));
+  _lemma_unchanged_node_vals_transitive h0 h0'' h1 (as_list h0 d1);
+  assume (dll_valid h1 d1);
+  assume (dll_valid h1 d2);
+  HST.pop_frame ();
+  let h11 = HST.get () in
+  B.popped_modifies h1 h11;
+  let loc = B.loc_region_only false (HS.get_tip h1) in
+  _lemma_nodelist_contained_in_unmodified_mem h1 h11 loc (as_list h11 d1);
+  _lemma_nodelist_contained_in_unmodified_mem h1 h11 loc (as_list h11 d2);
+  _lemma_nodelist_conn_in_unmodified_mem h1 h11 loc (as_list h11 d1);
+  _lemma_nodelist_conn_in_unmodified_mem h1 h11 loc (as_list h11 d2)
+
+#reset-options
+
 /// Automatic validity maintenance
 ///
 /// These are lemmas that you shouldn't really need to refer to
